Add more tests for SailTinyArm+SeqModel

ArchSemArm/tests/ArmSeqModelTest.v
@@ -4,10 +4,23 @@ From ASCommon Require Import CResult.
 
 
 
-(* Run EOR X0, X1, X2 at pc address 0x500, whose opcode is 0xca020020 *)
 Open Scope stdpp.
 Open Scope bv.
 
+(** Extract R0 in a Z on success to have something printable by Coq *)
+Definition r0_extract (a : Model.Res.t ∅ 1) : result string Z :=
+  match a with
+  | Model.Res.FinalState fs =>
+      let regs : registerMap := fs.(MState.regs) !!! 0%fin in
+      let r0 : bv 64 := regs R0 in
+      Ok (bv_unsigned r0)
+  | Model.Res.Error s => Error s
+  | Model.Res.Unspecified e => match e with end
+  end.
+
+
+(* Run EOR X0, X1, X2 at pc address 0x500, whose opcode is 0xca020020 *)
+Module EOR.
 Equations init_reg : registerMap:=
   init_reg (GReg (R_bitvector_64 _PC)) := 0x500;
   init_reg (GReg (R_bitvector_64 R0)) := 0x0;
@@ -29,19 +42,68 @@ Definition initState :=
     MState.termCond := termCond |}.
 Definition test_results := sequential_modelc None 2 sail_tiny_arm_sem 1%nat initState.
 
-(** Extract R0 on success to have something printable by Coq *)
-Definition result_extract (a : Model.Res.t ∅ 1) : result string Z :=
-  match a with
-  | Model.Res.FinalState fs =>
-      let x := (fs.(MState.regs)) in
-      let y : registerMap := x !!! 0%fin in
-      let z : bv 64 := y R0 in
-      Ok (bv_unsigned z)
-  | Model.Res.Error s => Error s
-  | Model.Res.Unspecified e => Error "hey"
-  end.
 
-Goal result_extract <$> test_results = Listset [Ok 0x110%Z].
+Goal r0_extract <$> test_results = Listset [Ok 0x110%Z].
   vm_compute (_ <$> _).
   reflexivity.
 Qed.
+End EOR.
+
+Module LDR. (* LDR X0, [X1, X0] at 0x500, loading from 0x1000 *)
+Equations init_reg : registerMap:=
+  init_reg (GReg (R_bitvector_64 _PC)) := 0x500;
+  init_reg (GReg (R_bitvector_64 R0)) := 0x1000;
+  init_reg _ := 0x0.
+
+Equations init_mem : memoryMap:=
+  init_mem 0x500 := 0x20; (* 0010 0000 *)
+  init_mem 0x501 := 0x68; (* 0110 1000 *)
+  init_mem 0x502 := 0x60; (* 0110 0000 *)
+  init_mem 0x503 := 0xF8; (* 1111 1000 *)
+  init_mem 0x1000 := 0x2a;
+  init_mem _ := 0x00.
+
+Definition termCond : terminationCondition 1 := (λ tid rm, rm _PC =? (0x504 : bv 64)).
+
+Definition initState :=
+  {| MState.state := {| MState.memory := init_mem; MState.regs := [# init_reg] |};
+    MState.termCond := termCond |}.
+Definition test_results := sequential_modelc None 2 sail_tiny_arm_sem 1%nat initState.
+
+Goal r0_extract <$> test_results = Listset [Ok 0x2a%Z].
+  vm_compute (_ <$> _).
+  reflexivity.
+Qed.
+End LDR.
+
+Module STRLDR. (* STR X2, [X1, X0]; LDR X0, [X1, X0] at 0x500, using address 0x1100 *)
+  Equations init_reg : registerMap:=
+    init_reg (GReg (R_bitvector_64 _PC)) := 0x500;
+    init_reg (GReg (R_bitvector_64 R0)) := 0x1000;
+    init_reg (GReg (R_bitvector_64 R1)) := 0x100;
+    init_reg (GReg (R_bitvector_64 R2)) := 0x2a;
+    init_reg _ := 0x0.
+
+  Equations init_mem : memoryMap:=
+    init_mem 0x500 := 0x22; (* 0010 0010 *)
+    init_mem 0x501 := 0x68; (* 0110 1000 *)
+    init_mem 0x502 := 0x20; (* 0010 0000 *)
+    init_mem 0x503 := 0xF8; (* 1111 1000 *)
+    init_mem 0x504 := 0x20; (* 0010 0000 *)
+    init_mem 0x505 := 0x68; (* 0110 1000 *)
+    init_mem 0x506 := 0x60; (* 0110 0000 *)
+    init_mem 0x507 := 0xF8; (* 1111 1000 *)
+    init_mem _ := 0x00.
+
+  Definition termCond : terminationCondition 1 := (λ tid rm, rm _PC =? (0x508 : bv 64)).
+
+  Definition initState :=
+    {| MState.state := {| MState.memory := init_mem; MState.regs := [# init_reg] |};
+      MState.termCond := termCond |}.
+  Definition test_results := sequential_modelc None 2 sail_tiny_arm_sem 1%nat initState.
+
+  Goal r0_extract <$> test_results = Listset [Ok 0x2a%Z].
+    vm_compute (_ <$> _).
+    reflexivity.
+  Qed.
+End STRLDR.
